Day 5 part 2: tail-recursive soln with proofs

Day5_2.lean
@@ -2,9 +2,28 @@ structure Range where
   lower: Nat
   upper: Nat
   h: lower <= upper
-deriving Repr, Ord
+deriving Repr
 
-instance: LE Range where le a b := (compare a b).isLE
+instance: Ord Range where compare a b := compare a.lower b.lower
+instance: LE Range := leOfOrd
+instance: LT Range := ltOfOrd
+
+@[grind =]
+theorem Range.le_lower (a b: Range) :
+    (a <= b) = (a.lower <= b.lower) := by 
+  unfold LE.le instLERange leOfOrd instLENat compare instOrdRange compare instOrdNat compareOfLessAndEq Ordering.isLE
+  grind only [cases Or]
+
+@[grind =]
+theorem Range.lt_lower (a b: Range) :
+    (a < b) = (a.lower < b.lower) := by 
+  unfold LT.lt instLTRange ltOfOrd instLTNat compare instOrdRange compare instOrdNat compareOfLessAndEq
+  simp
+  grind only [cases Or]
+
+@[grind =]
+theorem Range.le_lt (a b: Range) : (a < b) = ¬(b <= a) := by grind
+
 instance: Inhabited Range where default := ⟨0, 0, by omega⟩
 def Range.size (r: Range) := r.upper - r.lower + 1
 
@@ -13,22 +32,46 @@ structure RangeSet where
   h: ranges.Pairwise fun a b => a.upper < b.lower
 
 instance: Inhabited RangeSet where default := ⟨[], List.Pairwise.nil⟩
+instance: Membership Range RangeSet where
+  mem rs := Membership.mem rs.ranges
+
+abbrev Sorted [LE α] (xs: List α): Prop := xs.Pairwise (· <= ·)
 
 def RangeSet.ofRanges (ranges: List Range): RangeSet :=
-  let rs := ranges.mergeSort (· <= ·)
+  let rs := ranges.mergeSort
+  have h: Sorted rs := by grind [List.sorted_mergeSort]
+
+  let rec build (done: RangeSet) (current: Range) (rest: List Range) 
+      (h_rest: Sorted rest)
+      (h1: (r: Range) -> r ∈ done.ranges -> r.upper < current.lower)
+      (h2: (r: Range) -> r ∈ rest -> current <= r): RangeSet :=
+    let rs := RangeSet.mk (done.ranges ++ [current]) <| by
+      simp [List.pairwise_append, done.h]
+      grind only [→ List.Pairwise.of_cons]
+    match rest with
+    | [] => rs
+    | x::xs => 
+      if h: current.upper >= x.lower then
+        let nc: Range := ⟨
+          current.lower, max current.upper x.upper,
+          by have := current.h; omega
+        ⟩
+        build done nc xs 
+          (h_rest := by grind only [!List.Pairwise.of_cons])
+          (h1 := by grind)
+          (h2 := by grind)
+      else
+        build rs x xs
+          (h_rest := by grind only [!List.Pairwise.of_cons])
+          (h1 := by have := current.h; grind)
+          (h2 := by grind [List.pairwise_cons])
+
   match rs with
   | [] => default
-  | first::rest => Id.run do
-      let mut out: List Range := []
-      let mut a := first
-      for b in rest do
-        if a.upper >= b.lower then 
-          a := ⟨a.lower, max a.upper b.upper, by sorry⟩
-        else
-          out := out.append [a]
-          a := b
-      out := out.append [a]
-      ⟨out, by sorry⟩
+  | x::xs => build default x xs 
+    (h_rest := by grind only [→ List.Pairwise.of_cons])
+    (h1 := fun r h => absurd h List.not_mem_nil)
+    (h2 := by grind [List.pairwise_cons])
 
 def parseRange (s: String): Range :=
   let parts := s.splitOn "-" |>.map String.toNat!
@@ -43,4 +86,3 @@ def main : IO Unit := do
   let rangeset := RangeSet.ofRanges ranges
   let answer := rangeset.ranges.map Range.size |>.sum
   IO.println answer
-
